# 第一节

![%E7%AC%AC%E4%B8%80%E8%8A%82%20f5b6678d5bd94667a63fa8e1ab462922/IMG_20210426_133744-01.jpeg](%E7%AC%AC%E4%B8%80%E8%8A%82%20f5b6678d5bd94667a63fa8e1ab462922/IMG_20210426_133744-01.jpeg)

$$\begin{aligned}解：\\&①AB\overline{C}\\&②AB\overline{C}+A\overline{B}C+\overline{A}BC\\&③\overline{AB}C+\overline{A}B\overline{C}+\overline{AB}C\\&④\Omega-ABC\end{aligned}$$

---

![%E7%AC%AC%E4%B8%80%E8%8A%82%20f5b6678d5bd94667a63fa8e1ab462922/IMG_20210426_133744-02.jpeg](%E7%AC%AC%E4%B8%80%E8%8A%82%20f5b6678d5bd94667a63fa8e1ab462922/IMG_20210426_133744-02.jpeg)

①

$$\begin{aligned}AB+\overline{A}B&=(A\cap\overline{A})\cup B\\&=\Phi\cup B\\&=B\end{aligned}$$

②

$$\begin {aligned}A\overline{B}+\overline{A}B+\overline{A}\,\overline{B}&=A\overline{B}+\overline{A}(B\cup \overline{B})\\&=A\overline{B}+\overline{A}\cup \Omega\\&=A\overline{B}+\overline{A}\\&=(A\cup \overline{A})(\overline{B}\cup \overline{A})\\&=\overline{AB}
\end{aligned}$$

③

$$\begin{aligned}(A\cup \overline{B})(\overline{A}\cup\overline{B})&=\overline{B}(A\cup\overline{A})\\&=\overline{B}\Omega\\&=\overline{B}\end{aligned}$$

④

$$\begin{aligned}(A\cup B)(A-B)&=(A\cup B)A\overline{B}\\&=AA\overline{B}\cup AB\overline{B}\\&=A\overline{B}\cup \Phi\\&=A\overline{B}\end{aligned}$$